---
title: '  Trigonometric Identities '
weight: 1 
---



# Trigonometric Identities

For all real values of {{< katex >}}\theta{{< /katex >}}, we have the following three identities.
(i) {{< katex >}}\sin ^{2} \theta+\cos ^{2} \theta=1{{< /katex >}}
(ii) {{< katex >}}1+\tan ^{2} \theta=\sec ^{2} \theta{{< /katex >}}
(iii) {{< katex >}}1+\cot ^{2} \theta=\operatorname{cosec}^{2} \theta{{< /katex >}}

These identities are termed as three fundamental identities of trigonometry.

We will now prove them as follows.

| Picture | Identity | Proof |
| :---: | :---: | :---: |
| Fig. 6.3 | {{< katex >}}\sin ^{2} \theta+\cos ^{2} \theta=1{{< /katex >}} | In the right angled {{< katex >}}\triangle O M P{{< /katex >}}, we have <br> {{< katex >}}\frac{O M}{O P}=\cos \theta, \frac{P M}{O P}=\sin \theta \ldots(1){{< /katex >}} <br> By Pythagoras theorem <br> {{< katex >}}M P^{2}+O M^{2}=O P^{2} \ldots(2){{< /katex >}} <br> Dividing each term on both sides of (2) by <br> {{< katex >}}O P^{2},(\because O P \neq 0){{< /katex >}} we get, <br> {{< katex >}}\frac{M P^{2}}{O P^{2}}+\frac{O M^{2}}{O P^{2}}=\frac{O P^{2}}{O P^{2}}{{< /katex >}} <br> {{< katex >}}\Rightarrow\left(\frac{M P}{O P}\right)^{2}+\left(\frac{O M}{O P}\right)^{2}=\left(\frac{O P}{O P}\right)^{2}{{< /katex >}} <br> From {{< katex >}}(1),(\sin \theta)^{2}+(\cos \theta)^{2}=1^{2}{{< /katex >}} <br> Hence {{< katex >}}\sin ^{2} \theta+\cos ^{2} \theta=1{{< /katex >}} <br> In the right angled {{< katex >}}\triangle O M P{{< /katex >}}, we have <br> {{< katex >}}\frac{M P}{O M}=\tan \theta, \quad \frac{O P}{O M}=\sec \theta \quad \ldots{{< /katex >}} (3) |

{{< katex >}}
\begin{aligned}
& \text { From (2), } M P^{2}+O M^{2}=O P^{2} \\
& \text { Dividing each term on both sides of (2) by } \\
& O M^{2},(\because O M \neq 0) \text { we get, } \\
& 1+\tan ^{2} \theta=\sec ^{2} \theta \quad \overline{O M^{2}}+\frac{M^{2}}{O M^{2}}=\frac{O P^{2}}{O M^{2}} \\
& \Rightarrow\left(\frac{M P}{O M}\right)^{2}+\left(\frac{O M}{O M}\right)^{2}=\left(\frac{O P}{O M}\right)^{2} \\
& \text { From }(3),(\tan \theta)^{2}+1^{2}=(\sec \theta)^{2} \\
& \text { Hence } 1+\tan ^{2} \theta=\sec ^{2} \theta \text {. } \\
& 1+\cot ^{2} \theta=\operatorname{cosec}^{2} \theta \\
& \frac{M P^{2}}{M P^{2}}+\frac{O M^{2}}{M P^{2}}=\frac{O P^{2}}{M P^{2}} \\
& \Rightarrow\left(\frac{M P}{M P}\right)^{2}+\left(\frac{O M}{M P}\right)^{2}=\left(\frac{O P}{M P}\right)^{2}
\end{aligned}
{{< /katex >}}

These identities can also be rewritten as follows.

 **Identity**

 **Equal forms**

{{< katex >}}
\begin{array}{l|l}
\sin ^{2} \theta+\cos ^{2} \theta=1 & \sin ^{2} \theta=1-\cos ^{2} \theta \text { (or) } \cos ^{2} \theta=1-\sin ^{2} \theta \\
1+\tan ^{2} \theta=\sec ^{2} \theta & \tan ^{2} \theta=\sec ^{2} \theta-1 \text { (or) } \sec ^{2} \theta-\tan ^{2} \theta=1 \\
1+\cot ^{2} \theta=\operatorname{cosec}^{2} \theta & \cot ^{2} \theta=\operatorname{cosec}^{2} \theta-1 \text { (or) } \operatorname{cosec}^{2} \theta-\cot ^{2} \theta=1
\end{array}
{{< /katex >}}

 **Note**

Though the above identities are true for any angle {{< katex >}}\theta{{< /katex >}}, we will consider the six trigonometric ratios only for {{< katex >}}0^{\circ}<\theta<90^{\circ}{{< /katex >}}

 **Activity 1**

Take a white sheet of paper. Construct two perpendicular lines {{< katex >}}O X, O Y{{< /katex >}} which meet at {{< katex >}}O{{< /katex >}}, as shown in the Fig. 6.4(a).

Considering {{< katex >}}O X{{< /katex >}} as {{< katex >}}X{{< /katex >}} axis, {{< katex >}}O Y{{< /katex >}} as {{< katex >}}Y{{< /katex >}} axis.

We will verify the values of {{< katex >}}\sin \theta{{< /katex >}} and {{< katex >}}\cos \theta{{< /katex >}} for certain angles {{< katex >}}\theta{{< /katex >}}.

Let {{< katex >}}\theta=30^{\circ}{{< /katex >}}

Construct a line segment {{< katex >}}O A{{< /katex >}} of any length such that {{< katex >}}\angle A O X=30^{\circ}{{< /katex >}}, as shown in the Fig. 6.4(b).

Draw a perpendicular from {{< katex >}}A{{< /katex >}} to {{< katex >}}O X{{< /katex >}}, meeting at {{< katex >}}B{{< /katex >}}.

![fig.6.4(a)](fig.6.4(a).png)

Now using scale, measure the lengths of {{< katex >}}A B, O B{{< /katex >}} and {{< katex >}}O A{{< /katex >}}.

Find the ratios {{< katex >}}\frac{A B}{O A}, \frac{O B}{O A}{{< /katex >}} and {{< katex >}}\frac{A B}{O B}{{< /katex >}}.

What do you get? Can you compare these values with the trigonometric table values? What is your conclusion? Carry out the same procedure for {{< katex >}}\theta=45^{\circ}{{< /katex >}} and {{< katex >}}\theta=60^{\circ}{{< /katex >}}. What are your conclusions?

![fig.6.4(b)](fig.6.4(b).png)

Fig. 6.4(b)

**Example 6.1** Prove that {{< katex >}}\tan ^{2} \theta-\sin ^{2} \theta=\tan ^{2} \theta \sin ^{2} \theta{{< /katex >}}

_Solution_ {{< katex >}}\tan ^{2} \theta-\sin ^{2} \theta=\tan ^{2} \theta-\frac{\sin ^{2} \theta}{\cos ^{2} \theta} \cdot \cos ^{2} \theta{{< /katex >}}

{{< katex >}}
=\tan ^{2} \theta\left(1-\cos ^{2} \theta\right)=\tan ^{2} \theta \sin ^{2} \theta
{{< /katex >}}

**Example 6.2** Prove that {{< katex >}}\frac{\sin A}{1+\cos A}=\frac{1-\cos A}{\sin A}{{< /katex >}}

_Solution_ {{< katex >}}\frac{\sin A}{1+\cos A}=\frac{\sin A}{1+\cos A} \times \frac{1-\cos A}{1-\cos A} \quad{{< /katex >}} [multiply numerator and denominator by the conjugate of {{< katex >}}1+\cos A{{< /katex >}} ]

{{< katex >}}
\begin{aligned}
& =\frac{\sin A(1-\cos A)}{(1+\cos A)(1-\cos A)}=\frac{\sin A(1-\cos A)}{1-\cos ^{2} A} \\
& =\frac{\sin A(1-\cos A)}{\sin ^{2} A}=\frac{1-\cos A}{\sin A}
\end{aligned}
{{< /katex >}}

**Example 6.3** Prove that {{< katex >}}1+\frac{\cot ^{2} \theta}{1+\operatorname{cosec} \theta}=\operatorname{cosec} \theta{{< /katex >}}

_Solution_ {{< katex >}}1+\frac{\cot ^{2} \theta}{1+\operatorname{cosec} \theta}=1+\frac{\operatorname{cosec}^{2} \theta-1}{\operatorname{cosec} \theta+1} \quad\left[\because \operatorname{cosec}^{2} \theta-1=\cot ^{2} \theta\right]{{< /katex >}}

{{< katex >}}
\begin{aligned}
& =1+\frac{(\operatorname{cosec} \theta+1)(\operatorname{cosec} \theta-1)}{\operatorname{cosec} \theta+1} \\
& =1+(\operatorname{cosec} \theta-1)=\operatorname{cosec} \theta
\end{aligned}
{{< /katex >}}

**Example 6.4** Prove that {{< katex >}}\sec \theta-\cos \theta=\tan \theta \sin \theta{{< /katex >}}

_Solution_ {{< katex >}}\sec \theta-\cos \theta \quad=\frac{1}{\cos \theta}-\cos \theta=\frac{1-\cos ^{2} \theta}{\cos \theta}{{< /katex >}}

{{< katex >}}
\begin{aligned}
& =\frac{\sin ^{2} \theta}{\cos \theta} \quad\left[\because 1-\cos ^{2} \theta=\sin ^{2} \theta\right] \\
& =\frac{\sin \theta}{\cos \theta} \times \sin \theta=\tan \theta \sin \theta
\end{aligned}
{{< /katex >}}

**Example 6.5** Prove that {{< katex >}}\sqrt{\frac{1+\cos \theta}{1-\cos \theta}}=\operatorname{cosec} \theta+\cot \theta{{< /katex >}}

_Solution_ {{< katex >}}\sqrt{\frac{1+\cos \theta}{1-\cos \theta}}=\sqrt{\frac{1+\cos \theta}{1-\cos \theta} \times \frac{1+\cos \theta}{1+\cos \theta}}{{< /katex >}} [multiply numerator and denominator

{{< katex >}}
\begin{aligned}
& =\sqrt{\frac{(1+\cos \theta)^{2}}{1-\cos ^{2} \theta}}=\frac{1+\cos \theta}{\sqrt{\sin ^{2} \theta}} \quad\left[\because \sin ^{2} \theta+\cos ^{2} \theta=1\right] \\
& =\frac{1+\cos \theta}{\sin \theta}=\operatorname{cosec} \theta+\cot \theta
\end{aligned}
{{< /katex >}}

**Example 6.6** Prove that {{< katex >}}\frac{\sec \theta}{\sin \theta}-\frac{\sin \theta}{\cos \theta}=\cot \theta{{< /katex >}}

_Solution_ {{< katex >}}\frac{\sec \theta}{\sin \theta}-\frac{\sin \theta}{\cos \theta}=\frac{\frac{1}{\cos \theta}}{\sin \theta}-\frac{\sin \theta}{\cos \theta}=\frac{1}{\sin \theta \cos \theta}-\frac{\sin \theta}{\cos \theta}{{< /katex >}}

{{< katex >}}
=\frac{1-\sin ^{2} \theta}{\sin \theta \cos \theta}=\frac{\cos ^{2} \theta}{\sin \theta \cos \theta}=\cot \theta
{{< /katex >}}

**Example 6.7** Prove that {{< katex >}}\sin ^{2} A \cos ^{2} B+\cos ^{2} A \sin ^{2} B+\cos ^{2} A \cos ^{2} B+\sin ^{2} A \sin ^{2} B=1{{< /katex >}}

_Solution_ {{< katex >}}\sin ^{2} A \cos ^{2} B+\cos ^{2} A \sin ^{2} B+\cos ^{2} A \cos ^{2} B+\sin ^{2} A \sin ^{2} B{{< /katex >}}

{{< katex >}}
\begin{aligned}
& =\sin ^{2} A \cos ^{2} B+\sin ^{2} A \sin ^{2} B+\cos ^{2} A \sin ^{2} B+\cos ^{2} A \cos ^{2} B \\
& =\sin ^{2} A\left(\cos ^{2} B+\sin ^{2} B\right)+\cos ^{2} A\left(\sin ^{2} B+\cos ^{2} B\right) \\
& =\sin ^{2} A(1)+\cos ^{2} A(1) \quad\left(\because \sin ^{2} B+\cos ^{2} B=1\right) \\
& =\sin ^{2} A+\cos ^{2} A=1
\end{aligned}
{{< /katex >}}

**Example 6.8** If {{< katex >}}\cos \theta+\sin \theta=\sqrt{2} \cos \theta{{< /katex >}}, then prove that {{< katex >}}\cos \theta-\sin \theta=\sqrt{2} \sin \theta{{< /katex >}}

_Solution_

{{< katex >}}
\text { Now, } \cos \theta+\sin \theta=\sqrt{2} \cos \theta \text {. }
{{< /katex >}}

Squaring both sides,

{{< katex >}}
\begin{aligned}
(\cos \theta+\sin \theta)^{2} & =(\sqrt{2} \cos \theta)^{2} \\
\cos ^{2} \theta+\sin ^{2} \theta+2 \sin \theta \cos \theta & =2 \cos ^{2} \theta
\end{aligned}
{{< /katex >}}

{{< katex >}}
\begin{aligned}
2 \cos ^{2} \theta-\cos ^{2} \theta-\sin ^{2} \theta & =2 \sin \theta \cos \theta \\
\cos ^{2} \theta-\sin ^{2} \theta & =2 \sin \theta \cos \theta \\
(\cos \theta+\sin \theta)(\cos \theta-\sin \theta) & =2 \sin \theta \cos \theta \\
\cos \theta-\sin \theta=\frac{2 \sin \theta \cos \theta}{\cos \theta+\sin \theta} & =\frac{2 \sin \theta \cos \theta}{\sqrt{2} \cos \theta} \quad[\because \cos \theta+\sin \theta=\sqrt{2} \cos \theta] \\
& =\sqrt{2} \sin \theta
\end{aligned}
{{< /katex >}}

Therefore, {{< katex >}}\cos \theta-\sin \theta=\sqrt{2} \sin \theta{{< /katex >}}.

**Example 6.9** Prove that {{< katex >}}(\operatorname{cosec} \theta-\sin \theta)(\sec \theta-\cos \theta)(\tan \theta+\cot \theta)=1{{< /katex >}}

_Solution_ {{< katex >}}(\operatorname{cosec} \theta-\sin \theta)(\sec \theta-\cos \theta)(\tan \theta+\cot \theta){{< /katex >}}

{{< katex >}}
\begin{aligned}
& =\left(\frac{1}{\sin \theta}-\sin \theta\right)\left(\frac{1}{\cos \theta}-\cos \theta\right)\left(\frac{\sin \theta}{\cos \theta}+\frac{\cos \theta}{\sin \theta}\right) \\
& =\frac{1-\sin ^{2} \theta}{\sin \theta} \times \frac{1-\cos ^{2} \theta}{\cos \theta} \times \frac{\sin ^{2} \theta+\cos ^{2} \theta}{\sin \theta \cos \theta} \\
& =\frac{\cos ^{2} \theta \sin ^{2} \theta \times 1}{\sin ^{2} \theta \cos ^{2} \theta}=1
\end{aligned}
{{< /katex >}}

**Example 6.10** Prove that {{< katex >}}\frac{\sin A}{1+\cos A}+\frac{\sin A}{1-\cos A}=2 \operatorname{cosec} A{{< /katex >}}.

_Solution_ {{< katex >}}\frac{\sin A}{1+\cos A}+\frac{\sin A}{1-\cos A}{{< /katex >}}

{{< katex >}}
\begin{aligned}
& =\frac{\sin A(1-\cos A)+\sin A(1+\cos A)}{(1+\cos A)(1-\cos A)} \\
& =\frac{\sin A-\sin A \cos A+\sin A+\sin A \cos A}{1-\cos ^{2} A} \\
& =\frac{2 \sin A}{1-\cos ^{2} A}=\frac{2 \sin A}{\sin ^{2} A}=2 \operatorname{cosec} \mathrm{A}
\end{aligned}
{{< /katex >}}

**Example 6.11** If {{< katex >}}\operatorname{cosec} \theta+\cot \theta=P{{< /katex >}}, then prove that {{< katex >}}\cos \theta=\frac{P^{2}-1}{P^{2}+1}{{< /katex >}}

_Solution_ Given {{< katex >}}\operatorname{cosec} \theta+\cot \theta=P{{< /katex >}}

{{< katex >}}
\begin{aligned}
\operatorname{cosec}^{2} \theta-\cot ^{2} \theta & =1 \text { (identity) } \\
\operatorname{cosec} \theta-\cot \theta & =\frac{1}{\operatorname{cosec} \theta+\cot \theta} \\
\operatorname{cosec} \theta-\cot \theta & =\frac{1}{P}
\end{aligned}
{{< /katex >}}

Adding (1) and (2) we get, {{< katex >}}\quad 2 \operatorname{cosec} \theta=P+\frac{1}{P}{{< /katex >}}

{{< katex >}}
2 \operatorname{cosec} \theta=\frac{P^{2}+1}{P}
{{< /katex >}}

Subtracting (2) from (1), we get, {{< katex >}}2 \cot \theta=P-\frac{1}{P}{{< /katex >}}[^0]

{{< katex >}}
2 \cot \theta=\frac{P^{2}-1}{P}
{{< /katex >}}

Dividing (4) by (3) we get, {{< katex >}}\frac{2 \cot \theta}{2 \operatorname{cosec} \theta}=\frac{P^{2}-1}{P} \times \frac{P}{P^{2}+1} \Rightarrow \cos \theta=\frac{P^{2}-1}{P^{2}+1}{{< /katex >}}

**Example 6.12** Prove that {{< katex >}}\tan ^{2} A-\tan ^{2} B=\frac{\sin ^{2} A-\sin ^{2} B}{\cos ^{2} A \cos ^{2} B}{{< /katex >}}

_Solution_ {{< katex >}}\tan ^{2} A-\tan ^{2} B=\frac{\sin ^{2} A}{\cos ^{2} A}-\frac{\sin ^{2} B}{\cos ^{2} B}{{< /katex >}}

{{< katex >}}
\begin{aligned}
& =\frac{\sin ^{2} A \cos ^{2} B-\sin ^{2} B \cos ^{2} A}{\cos ^{2} A \cos ^{2} B} \\
& =\frac{\sin ^{2} A\left(1-\sin ^{2} B\right)-\sin ^{2} B\left(1-\sin ^{2} A\right)}{\cos ^{2} A \cos ^{2} B} \\
& =\frac{\sin ^{2} A-\sin ^{2} A \sin ^{2} B-\sin ^{2} B+\sin ^{2} A \sin ^{2} B}{\cos ^{2} A \cos ^{2} B}=\frac{\sin ^{2} A-\sin ^{2} B}{\cos ^{2} A \cos ^{2} B}
\end{aligned}
{{< /katex >}}

**Example 6.13** Prove that {{< katex >}}\left(\frac{\cos ^{3} A-\sin ^{3} A}{\cos A-\sin A}\right)-\left(\frac{\cos ^{3} A+\sin ^{3} A}{\cos A+\sin A}\right)=2 \sin A \cos A{{< /katex >}}

_Solution_ {{< katex >}}\left(\frac{\cos ^{3} A-\sin ^{3} A}{\cos A-\sin A}\right)-\left(\frac{\cos ^{3} A+\sin ^{3} A}{\cos A+\sin A}\right){{< /katex >}}

{{< katex >}}
\begin{aligned}
& =\left(\frac{(\cos A-\sin A)\left(\cos ^{2} A+\sin ^{2} A+\cos A \sin A\right)}{\cos A-\sin A}\right)\left[\begin{array}{r}
\because a^{3}-b^{3}=(a-b)\left(a^{2}+b^{2}+a b\right) \\
a^{3}+b^{3}=(a+b)\left(a^{2}+b^{2}-a b\right)
\end{array}\right] \\
& -\left(\frac{(\cos A+\sin A)\left(\cos ^{2} A+\sin ^{2} A-\cos A \sin A\right)}{\cos A+\sin A}\right) \\
& =(1+\cos A \sin A)-(1-\cos A \sin A) \\
& =2 \cos A \sin A
\end{aligned}
{{< /katex >}}

**Example 6.14** Prove that {{< katex >}}\frac{\sin A}{\sec A+\tan A-1}+\frac{\cos A}{\operatorname{cosec} A+\cot A-1}=1{{< /katex >}}

_Solution_ {{< katex >}}\frac{\sin A}{\sec A+\tan A-1}+\frac{\cos A}{\operatorname{cosec} \mathrm{A}+\cot A-1}{{< /katex >}}

{{< katex >}}
\begin{aligned}
& =\frac{\sin A(\operatorname{cosec} A+\cot A-1)+\cos A(\sec A+\tan A-1)}{(\sec A+\tan A-1)(\operatorname{cosec} A+\cot A-1)} \\
& =\frac{\sin A \operatorname{cosec} A+\sin A \cot A-\sin A+\cos A \sec A+\cos A \tan A-\cos A}{(\sec A+\tan A-1)(\operatorname{cosec} A+\cot A-1)} \\
& =\frac{1+\cos A-\sin A+1+\sin A-\cos A}{\left(\frac{1}{\cos A}+\frac{\sin A}{\cos A}-1\right)\left(\frac{1}{\sin A}+\frac{\cos A}{\sin A}-1\right)}
\end{aligned}
{{< /katex >}}

{{< katex >}}
\begin{aligned}
& =\frac{2}{\left(\frac{1+\sin A-\cos A}{\cos A}\right)\left(\frac{1+\cos A-\sin A}{\sin A}\right)} \\
& =\frac{2 \sin A \cos A}{(1+\sin A-\cos A)(1+\cos A-\sin A)} \\
& =\frac{2 \sin A \cos A}{[1+(\sin A-\cos A)][1-(\sin A-\cos A)]}=\frac{2 \sin A \cos A}{1-(\sin A-\cos A)^{2}} \\
& =\frac{2 \sin A \cos A}{1-\left(\sin ^{2} A+\cos ^{2} A-2 \sin A \cos A\right)}=\frac{2 \sin A \cos A}{1-(1-2 \sin A \cos A)} \\
& =\frac{2 \sin A \cos A}{1-1+2 \sin A \cos A}=\frac{2 \sin A \cos A}{2 \sin A \cos A}=1 .
\end{aligned}
{{< /katex >}}

**Example 6.15** Show that {{< katex >}}\left(\frac{1+\tan ^{2} A}{1+\cot ^{2} A}\right)=\left(\frac{1-\tan A}{1-\cot A}\right)^{2}{{< /katex >}}

_Solution_

 LHS

{{< katex >}}
\begin{aligned}
\left(\frac{1+\tan ^{2} A}{1+\cot ^{2} A}\right) & =\frac{1+\tan ^{2} A}{1+\frac{1}{\tan ^{2} A}} \\
& =\frac{1+\tan ^{2} A}{\frac{\tan ^{2} A+1}{\tan ^{2} A}}=\tan ^{2} A \ldots
\end{aligned}
{{< /katex >}}

{{< katex >}}
\begin{aligned}
& \text { RHS } \\
& \left(\frac{1-\tan A}{1-\cot A}\right)^{2}=\left(\frac{1-\tan A}{1-\frac{1}{\tan A}}\right)^{2} \\
& =\left(\frac{1-\tan A}{\frac{\tan A-1}{\tan A}}\right)^{2}=(-\tan A)^{2}=\tan ^{2} A \ldots
\end{aligned}
{{< /katex >}}

From (1) and (2), {{< katex >}}\left(\frac{1+\tan ^{2} A}{1+\cot ^{2} A}\right)=\left(\frac{1-\tan A}{1-\cot A}\right)^{2}{{< /katex >}}

**Example 6.16** Prove that {{< katex >}}\frac{(1+\cot A+\tan A)(\sin A-\cos A)}{\sec ^{3} A-\cos e c^{3} A}=\sin ^{2} A \cos ^{2} A{{< /katex >}}

_Solution_ {{< katex >}}\frac{(1+\cot A+\tan A)(\sin A-\cos A)}{\sec ^{3} A-\operatorname{cosec} c^{3} A}{{< /katex >}}

{{< katex >}}
\begin{aligned}
& =\frac{\left(1+\frac{\cos A}{\sin A}+\frac{\sin A}{\cos A}\right)(\sin A-\cos A)}{(\sec A-\operatorname{cosec} A)\left(\sec ^{2} A+\sec A \operatorname{cosec} A+\operatorname{cosec} A\right)} \\
& =\frac{\frac{\left(\sin A \cos A+\cos ^{2} A+\sin ^{2} A\right)(\sin A-\cos A)}{\sin A \cos A}}{(\sec A-\operatorname{cosec} A)\left(\frac{1}{\cos ^{2} A}+\frac{1}{\cos A \sin A}+\frac{1}{\sin ^{2} A}\right)}
\end{aligned}
{{< /katex >}}

{{< katex >}}
\begin{aligned}
& =\frac{(\sin A \cos A+1)\left(\frac{\sin A}{\sin A \cos A}-\frac{\cos A}{\sin A \cos A}\right)}{(\sec A-\operatorname{cosec} A)\left(\frac{\sin ^{2} A+\sin A \cos A+\cos ^{2} A}{\sin ^{2} A \cos ^{2} A}\right)} \\
& =\frac{(\sin A \cos A+1)(\sec A-\cos e c A)}{(\sec A-\cos e c A)(1+\sin A \cos A)} \times \sin ^{2} A \cos ^{2} A=\sin ^{2} A \cos ^{2} A
\end{aligned}
{{< /katex >}}

**Example 6.17** If {{< katex >}}\frac{\cos ^{2} \theta}{\sin \theta}=p{{< /katex >}} and {{< katex >}}\frac{\sin ^{2} \theta}{\cos \theta}=q{{< /katex >}}, then prove that {{< katex >}}p^{2} q^{2}\left(p^{2}+q^{2}+3\right)=1{{< /katex >}}

_Solution_ We have {{< katex >}}\frac{\cos ^{2} \theta}{\sin \theta}=p \ldots{{< /katex >}}...(1) and {{< katex >}}\frac{\sin ^{2} \theta}{\cos \theta}=q{{< /katex >}}...

{{< katex >}}
\begin{aligned}
p^{2} q^{2}\left(p^{2}+q^{2}+3\right) & =\left(\frac{\cos ^{2} \theta}{\sin \theta}\right)^{2}\left(\frac{\sin ^{2} \theta}{\cos \theta}\right)^{2} \times\left[\left(\frac{\cos ^{2} \theta}{\sin \theta}\right)^{2}+\left(\frac{\sin ^{2} \theta}{\cos \theta}\right)^{2}+3\right][\text { from (1) and (2)] } \\
& =\left(\frac{\cos ^{4} \theta}{\sin ^{2} \theta}\right)\left(\frac{\sin ^{4} \theta}{\cos ^{2} \theta}\right) \times\left[\frac{\cos ^{4} \theta}{\sin ^{2} \theta}+\frac{\sin ^{4} \theta}{\cos ^{2} \theta}+3\right] \\
& =\left(\cos ^{2} \theta \times \sin ^{2} \theta\right) \times\left[\left(\frac{\cos ^{6} \theta+\sin ^{6} \theta+3 \sin ^{2} \theta \cos ^{2} \theta}{\sin ^{2} \theta \cos ^{2} \theta}\right)\right] \\
& =\cos ^{6} \theta+\sin ^{6} \theta+3 \sin ^{2} \theta \cos ^{2} \theta \\
& =\left(\cos ^{2} \theta\right)^{3}+\left(\sin ^{2} \theta\right)^{3}+3 \sin ^{2} \theta \cos ^{2} \theta \\
& =\left[\left(\cos ^{2} \theta+\sin ^{2} \theta\right)^{3}-3 \cos ^{2} \theta \sin ^{2} \theta\left(\cos ^{2} \theta+\sin ^{2} \theta\right)\right]+3 \sin ^{2} \theta \cos ^{2} \theta \\
& =1-3 \cos ^{2} \theta \sin ^{2} \theta(1)+3 \cos ^{2} \theta \sin ^{2} \theta=1
\end{aligned}
{{< /katex >}}

 **Progress Check** 

1. The number of trigonometric ratios is
2. {{< katex >}}1-\cos ^{2} \theta{{< /katex >}} is
3. {{< katex >}}(\sec \theta+\tan \theta)(\sec \theta-\tan \theta){{< /katex >}} is
4. {{< katex >}}(\cot \theta+\operatorname{cosec} \theta)(\cot \theta-\operatorname{cosec} \theta){{< /katex >}} is
5. {{< katex >}}\cos 60^{\circ} \sin 30^{\circ}+\cos 30^{\circ} \sin 60^{\circ}{{< /katex >}} is
6. {{< katex >}}\tan 60^{\circ} \cos 60^{\circ}+\cot 60^{\circ} \sin 60^{\circ}{{< /katex >}} is
7. {{< katex >}}\left(\tan 45^{\circ}+\cot 45^{\circ}\right)+\left(\sec 45^{\circ} \operatorname{cosec} 45^{\circ}\right){{< /katex >}} is
8. (i) {{< katex >}}\sec \theta=\operatorname{cosec} \theta{{< /katex >}} if {{< katex >}}\theta{{< /katex >}} is

(ii) {{< katex >}}\cot \theta=\tan \theta{{< /katex >}} if {{< katex >}}\theta{{< /katex >}} is

 **Exercise 6.1**

1. Prove the following identities.
(i) {{< katex >}}\cot \theta+\tan \theta=\sec \theta \operatorname{cosec} \theta{{< /katex >}}
(ii) {{< katex >}}\tan ^{4} \theta+\tan ^{2} \theta=\sec ^{4} \theta-\sec ^{2} \theta{{< /katex >}}
2. Prove the following identities.
(i) {{< katex >}}\frac{1-\tan ^{2} \theta}{\cot ^{2} \theta-1}=\tan ^{2} \theta{{< /katex >}}
(ii) {{< katex >}}\frac{\cos \theta}{1+\sin \theta}=\sec \theta-\tan \theta{{< /katex >}}
3. Prove the following identities.
(i) {{< katex >}}\sqrt{\frac{1+\sin \theta}{1-\sin \theta}}=\sec \theta+\tan \theta{{< /katex >}}
(ii) {{< katex >}}\sqrt{\frac{1+\sin \theta}{1-\sin \theta}}+\sqrt{\frac{1-\sin \theta}{1+\sin \theta}}=2 \sec \theta{{< /katex >}}
4. Prove the following identities.

(i) {{< katex >}}\sec ^{6} \theta=\tan ^{6} \theta+3 \tan ^{2} \theta \sec ^{2} \theta+1{{< /katex >}}

(ii) {{< katex >}}(\sin \theta+\sec \theta)^{2}+(\cos \theta+\operatorname{cosec} \theta)^{2}=1+(\sec \theta+\operatorname{cosec} \theta)^{2}{{< /katex >}}

5. Prove the following identities.
(i) {{< katex >}}\sec ^{4} \theta\left(1-\sin ^{4} \theta\right)-2 \tan ^{2} \theta=1{{< /katex >}}
(ii) {{< katex >}}\frac{\cot \theta-\cos \theta}{\cot \theta+\cos \theta}=\frac{\operatorname{cosec} \theta-1}{\operatorname{cosec} \theta+1}{{< /katex >}}
6. Prove the following identities.
(i) {{< katex >}}\frac{\sin A-\sin B}{\cos A+\cos B}+\frac{\cos A-\cos B}{\sin A+\sin B}=0{{< /katex >}}
(ii) {{< katex >}}\frac{\sin ^{3} A+\cos ^{3} A}{\sin A+\cos A}+\frac{\sin ^{3} A-\cos ^{3} A}{\sin A-\cos A}=2{{< /katex >}}
7. (i) If {{< katex >}}\sin \theta+\cos \theta=\sqrt{3}{{< /katex >}}, then prove that {{< katex >}}\tan \theta+\cot \theta=1{{< /katex >}}.

(ii) If {{< katex >}}\sqrt{3} \sin \theta-\cos \theta=0{{< /katex >}}, then show that {{< katex >}}\tan 3 \theta=\frac{3 \tan \theta-\tan ^{3} \theta}{1-3 \tan ^{2} \theta}{{< /katex >}}

8. (i) If {{< katex >}}\frac{\cos \alpha}{\cos \beta}=m{{< /katex >}} and {{< katex >}}\frac{\cos \alpha}{\sin \beta}=n{{< /katex >}}, then prove that {{< katex >}}\left(m^{2}+n^{2}\right) \cos ^{2} \beta=n^{2}{{< /katex >}}

(ii) If {{< katex >}}\cot \theta+\tan \theta=x{{< /katex >}} and {{< katex >}}\sec \theta-\cos \theta=y{{< /katex >}}, then prove that {{< katex >}}\left(x^{2} y\right)^{\frac{2}{3}}-\left(x y^{2}\right)^{\frac{2}{3}}=1{{< /katex >}}

9. (i) If {{< katex >}}\sin \theta+\cos \theta=p{{< /katex >}} and {{< katex >}}\sec \theta+\operatorname{cosec} \theta=q{{< /katex >}}, then prove that {{< katex >}}q\left(p^{2}-1\right)=2 p{{< /katex >}}

(ii) If {{< katex >}}\sin \theta\left(1+\sin ^{2} \theta\right)=\cos ^{2} \theta{{< /katex >}}, then prove that {{< katex >}}\cos ^{6} \theta-4 \cos ^{4} \theta+8 \cos ^{2} \theta=4{{< /katex >}}

10. If {{< katex >}}\frac{\cos \theta}{1+\sin \theta}=\frac{1}{a}{{< /katex >}}, then prove that {{< katex >}}\frac{a^{2}-1}{a^{2}+1}=\sin \theta{{< /katex >}}




